feat: Update links in `block.v`

CoqOfRust/revm/revm_context_interface/links/block.v
@@ -3,38 +3,78 @@ Require Import CoqOfRust.links.M.
 (* Require Import CoqOfRust.core.convert.links.mod. *)
 Require Import CoqOfRust.revm.links.dependencies.
 (* Require Import CoqOfRust.revm.revm_specification.links.hardfork. *)
-(* TODO: import for Address *)
+
+Module Address := dependencies.alloy_primitives.bits.links.address.Address.
 
 (* 
 #[auto_impl(&, &mut, Box, Arc)]
 pub trait Block {
     fn number(&self) -> u64;
-
     fn beneficiary(&self) -> Address;
-
     fn timestamp(&self) -> u64;
-
     fn gas_limit(&self) -> u64;
-
     fn basefee(&self) -> u64;
-
     fn difficulty(&self) -> U256;
-
     fn prevrandao(&self) -> Option<B256>;
-
     fn blob_excess_gas_and_price(&self) -> Option<BlobExcessGasAndPrice>;
-
     fn blob_gasprice(&self) -> Option<u128> {
         self.blob_excess_gas_and_price().map(|a| a.blob_gasprice)
     }
-
     fn blob_excess_gas(&self) -> Option<u64> {
         self.blob_excess_gas_and_price().map(|a| a.excess_blob_gas)
     }
 }
 *)
 Module Block. 
-  (* 
-    fn beneficiary(&self) -> Address;
-  *)
+  Parameter t : Set.
+
+  Definition Run_beneficiary (Self : Set) `{Link Self} : Set :=
+    {beneficiary @
+      IsTraitMethod.t "revm_context_interface::block::Block" [] [] (Φ Self) "beneficiary" beneficiary *
+      forall (self : Ref.t Pointer.Kind.Ref Self),
+        {{ beneficiary [] [] [ φ self ] 🔽 Address.t }}
+    }.
+
+  Record Run (Self : Set) `{Link Self} : Set := {
+    beneficiary : Run_beneficiary Self;
+  }.
 End Block. 
+
+(* 
+#[auto_impl(&, &mut, Box, Arc)]
+pub trait BlockGetter {
+    type Block: Block;
+
+    fn block(&self) -> &Self::Block;
+}
+*)
+Module BlockGetter.
+  Module Types.
+    Record t : Type := {
+      Block : Set;
+    }.
+
+    Class AreLinks (types : t) : Set := {
+      H_Block : Link types.(Block);
+    }.
+
+    Global Instance IsLinkBlock (types : t) (H : AreLinks types) : Link types.(Block) :=
+      H.(H_Block _).
+  End Types.
+
+  Definition Run_block (Self : Set) `{Link Self} : Set :=
+    {block @
+      IsTraitMethod.t "revm_context_interface::block::BlockGetter" [] [] (Φ Self) "block" block *
+      forall (self : Ref.t Pointer.Kind.Ref Self),
+        {{ block [] [] [ φ self ] 🔽 unit }}
+    }.
+
+  Record Run (Self : Set) `{Link Self} (types : Types.t)  `{Types.AreLinks types} : Set := {
+    Block_IsAssociated : 
+      IsTraitAssociatedType
+        "revm_context_interface::block::BlockGetter" [] [] (Φ Self)
+        "Block" (Φ types.(Types.Block));
+    run_Block_for_Block : Block.Run types.(Types.Block);
+    block : Run_block Self;
+  }.
+End BlockGetter.
